theories/interop/roots.v
@@ -1,0 +1,105 @@
+From Coq Require Import ssreflect.
+From stdpp Require Import strings gmap.
+From transfinite.base_logic.lib Require Import ghost_map ghost_var gen_heap.
+From iris.algebra Require Import gset.
+From iris.proofmode Require Import proofmode.
+From melocoton Require Import named_props iris_extra.
+From melocoton.interop Require Export basics basics_resources.
+From melocoton.c_interface Require Import defs resources.
+
+Section ROOTS.
+Context `{SI: indexT}.
+Context {Σ : gFunctors}.
+Context `{!heapG_C Σ}.
+Context `{!wrapperBasicsG Σ}.
+
+Definition ROOTS (θ : addr_map) (roots_m : roots_map) : iProp Σ :=
+  ∃ (memr: memory),
+    "GCrootspto" ∷ ([∗ map] a↦w ∈ memr, a O↦C w)
+  ∗ "%Hreprroots" ∷ ⌜repr_roots θ roots_m memr⌝
+  (* NOTE: it does not seem necessary to include [roots_are_live] here,
+     but at the same time, it is convenient to do so... *)
+  ∗ "%Hrootslive" ∷ ⌜roots_are_live θ roots_m⌝.
+
+Lemma ROOTS_live θ roots_m :
+  ROOTS θ roots_m -∗
+  ⌜roots_are_live θ roots_m⌝.
+Proof. by iNamed 1. Qed.
+
+Lemma ROOTS_valid θ roots_m mem :
+  ROOTS θ roots_m -∗
+  gen_heap_interp mem -∗
+  ⌜∃ privmem, repr_mem θ roots_m privmem mem⌝.
+Proof.
+  iNamed 1. iIntros "Hmem".
+  iDestruct (gen_heap_valid_big with "Hmem GCrootspto") as %(privmem & -> & Hdisj).
+  iPureIntro. do 2 eexists; split_and!; eauto.
+Qed.
+
+Lemma ROOTS_pto_notin θ roots_m a w :
+  ROOTS θ roots_m -∗
+  a ↦C w -∗
+  ⌜a ∉ dom roots_m⌝.
+Proof.
+  iIntros "Hr Hpto %H". iNamed "Hr". apply elem_of_dom in H as [? H].
+  edestruct repr_roots_lookup as (w' & ? & ?); eauto; simplify_eq.
+  iDestruct (big_sepM_lookup with "GCrootspto") as "Hpto'"; first done.
+  by iPoseProof (resources.mapsto_ne with "Hpto Hpto'") as "%HH".
+Qed.
+
+Lemma ROOTS_empty θ : ⊢ ROOTS θ ∅.
+Proof.
+  rewrite /ROOTS /named. iExists ∅. rewrite big_sepM_empty.
+  iPureIntro; split_and!; eauto.
+  - apply repr_roots_empty.
+  - apply roots_are_live_empty.
+Qed.
+
+Lemma ROOTS_update_θ θ θ' roots_m privmem mem mem' :
+  roots_are_live θ' roots_m →
+  repr_mem θ roots_m privmem mem →
+  repr_mem θ' roots_m privmem mem' →
+  ROOTS θ roots_m -∗
+  gen_heap_interp mem
+  ==∗
+  ROOTS θ' roots_m ∗
+  gen_heap_interp mem'.
+Proof.
+  intros Hlive (memr & Hrepr & Hdisj & ->) (memr' & Hrepr' & Hdisj' & ->).
+  iNamed 1. iIntros "Hmem".
+  pose proof (repr_roots_inj_2 _ _ _ _ Hrepr Hreprroots) as <-.
+  iMod (gen_heap_update_big memr memr' with "GCrootspto Hmem") as "[GCrootspto $]"; auto.
+  { rewrite -(repr_roots_dom _ _ _ Hreprroots) -(repr_roots_dom _ _ _ Hrepr')//. }
+  iModIntro. rewrite /ROOTS /named. iExists _. by iFrame.
+Qed.
+
+Lemma ROOTS_insert θ roots_m a lv w :
+  repr_lval θ lv w →
+  ROOTS θ roots_m -∗
+  a O↦C (Storing w) -∗
+  ROOTS θ (<[a := lv]> roots_m).
+Proof.
+  iIntros (Hrepr) "Hr Hpto". iDestruct (ROOTS_pto_notin with "Hr Hpto") as %Hdom.
+  iNamed "Hr".
+  iDestruct (big_sepM_insert with "[$GCrootspto $Hpto]") as "GCrootspto".
+  { apply not_elem_of_dom. erewrite <- repr_roots_dom; eauto. }
+  rewrite /ROOTS /named. iExists _. iFrame. iPureIntro. split.
+  - eapply repr_roots_insert; eauto.
+  - eapply roots_are_live_insert; eauto.
+Qed.
+
+Lemma ROOTS_delete θ roots_m a lv :
+  roots_m !! a = Some lv →
+  ROOTS θ roots_m -∗
+  ∃ w, ROOTS θ (delete a roots_m) ∗ a O↦C (Storing w) ∗ ⌜repr_lval θ lv w⌝.
+Proof.
+  intros Hr. iNamed 1.
+  edestruct repr_roots_lookup as (w & Hw & ?); eauto.
+  iDestruct (big_sepM_delete with "GCrootspto") as "[Hpto Hptos]"; first done.
+  iExists _.  iFrame "Hpto". iSplit; last done. rewrite /ROOTS /named.
+  iExists _. iFrame. iPureIntro. split.
+  - by eapply repr_roots_delete.
+  - by eapply roots_are_live_delete.
+Qed.
+
+End ROOTS.
